Clase3.Vec.fst
@@ -8,6 +8,10 @@ let vhd (#a:Type) (#n:pos) (xs : vec a n) : a =
   match xs with
   | VCons hd tl -> hd
 
+let vtl (#a:Type) (#n:pos) (xs : vec a n) : vec a (n-1) =
+  match xs with
+  | VCons hd tl -> tl
+
 let rec vidx (#a:Type) (#n:pos) (xs : vec a n) (i : nat{i < n}) : a =
   match xs with
   | VCons hd tl ->
@@ -15,20 +19,33 @@ let rec vidx (#a:Type) (#n:pos) (xs : vec a n) (i : nat{i < n}) : a =
     then hd
     else vidx tl (i-1)
 
-let vappend (#a:Type) (#n1 #n2 : nat) (xs : vec a n1) (ys : vec a n2) : vec a (n1 + n2) =
-  admit() (* completar *)
+let rec vappend (#a:Type) (#n1 #n2 : nat) (xs : vec a n1) (ys : vec a n2) : vec a (n1 + n2) =
+  match xs with
+  | VNil -> ys
+  | VCons hd tl -> VCons hd (vappend tl ys)
 
-let vupd (#a:Type) (#n:pos) (xs : vec a n) (i : nat{i < n}) (x : a) : vec a n =
-  admit() (* completar *)
+let rec vupd (#a:Type) (#n:pos) (xs : vec a n) (i : nat{i < n}) (x : a) : vec a n =
+  match i with
+  | 0 -> VCons x (vtl xs)
+  | _ -> VCons (vhd xs) (vupd (vtl xs) (i-1) x)
 
 (* Definir funciones similares para matrices. Se pueden
 usar las definiciones anteriores. *)
 
-let mat (a:Type) (m n : nat) : Type =
-  admit()
+type mat (a:Type) : nat-> nat -> Type =
+  | MRow : #n:nat -> vec a n -> mat a 1 n
+  | MCons : #m:nat -> #n:nat -> vec a n -> mat a m n -> mat a (m+1) n
   
-let matidx (#a:Type) (#m #n : nat) (ma : mat a m n) (i : nat{i < m}) (j : nat{j < n}) : a =
-  admit()
+let rec matidx (#a:Type) (#m #n : nat) (ma : mat a m n) (i : nat{i < m}) (j : nat{j < n}) : a =
+  match ma with
+  | MRow vs -> vidx vs j
+  | MCons vs ma' -> if i = 0
+                    then vidx vs j
+                    else matidx ma' (i-1) j
   
-let matupd (#a:Type) (#m #n : nat) (ma : mat a m n) (i : nat{i < m}) (j : nat{j < n}) (x : a) : mat a m n =
-  admit()
+let rec matupd (#a:Type) (#m #n : nat) (ma : mat a m n) (i : nat{i < m}) (j : nat{j < n}) (x : a) : mat a m n =
+  match ma with
+  | MRow vs -> MRow (vupd vs j x)
+  | MCons vs ma' -> if i = 0
+                    then MCons (vupd vs j x) ma'
+                    else MCons vs (matupd ma' (i-1) j x)
